---
title: "ç¾ä»£æ•°ç†çµ±è¨ˆå­¦ ç¬¬2ç«  æ¼”ç¿’å•é¡Œ å•4 è‡ªä½œè§£ç­”"
emoji: "ğŸ‘‹"
type: "tech"
topics: []
published: false
---

### $E[(X-t)^2]$ã®æœ€å°å€¤

$$
\begin{align*}
E[(X-t)^2] &= E[X^2 -2tX + t^2] \\
&= E[X^2] - E[2tX] + E[t^2] \\
&= E[X^2] - 2tE[X] + t^2
\end{align*}
$$

ã“ã‚Œã‚’$t$ã®å¼ã¨è¦‹ã‚‹ã¨ï¼Œ

$$
\begin{align*}
E[X^2] - 2tE[X] + t^2
&= t^2  - 2E[X] t + E[X^2] \\
&= t^2  - 2E[X] t + E[X]^2 - E[X]^2 + E[X^2] \\
&= (t - E[X])^2 - E[X]^2 + E[X^2]  \\
&= (t - E[X])^2 + E[X^2] - E[X]^2 \\
&= (t - E[X])^2 + V[X]
\end{align*}
$$

ã§ã‚ã‚Šï¼Œ$t=E[X]$ã®ã¨ãæœ€å°å€¤ã‚’å–ã‚‹ã“ã¨ãŒã‚ã‹ã‚‹ï¼


### $E[|X-t|]$ã®æœ€å°å€¤